checkpoint before update for ligo changes

src/contracts_coq/did_manager.v
@@ -31,53 +31,97 @@ Require map.
 Require String.
 
 Require did_manager_string.
+(* Require did_manager_michelson_string. *)
+
+(* Module raw. *)
+
+(* Import String. *)
+
+(* Definition did_manager_michelson_string : string := " *)
+(* parameter *)
+(*   (or (or (address %rotateAuthentication) (address %rotateOwner)) *)
+(*       (pair %rotateService (string %endpoint) (string %type_))); *)
+(* storage *)
+(*   (pair (pair (big_map %metadata string bytes) (address %owner)) *)
+(*         (pair (pair %service (string %endpoint) (string %type_)) *)
+(*               (address %verification_method))); *)
+(* code { UNPAIR; *)
+(*        SWAP; *)
+(*        UNPAIR; *)
+(*        UNPAIR; *)
+(*        SWAP; *)
+(*        DUP; *)
+(*        SENDER; *)
+(*        COMPARE; *)
+(*        EQ; *)
+(*        IF { SWAP; *)
+(*             DIP { DIG 2; *)
+(*                   IF_LEFT *)
+(*                     { IF_LEFT *)
+(*                         { SWAP; DIP { SWAP; UNPAIR; SWAP; DROP; PAIR } } *)
+(*                         { SWAP; DROP } } *)
+(*                     { SWAP; DIP { SWAP; DUP; CAR; DROP; CDR; SWAP; PAIR } } }; *)
+(*             AMOUNT; *)
+(*             PUSH mutez 0; *)
+(*             COMPARE; *)
+(*             EQ; *)
+(*             IF { PAIR; PAIR; NIL operation; PAIR } *)
+(*                { SWAP; FAILWITH } } *)
+(*           { FAILWITH } }". *)
+(* End raw. *)
 
 Module source.
   Definition contract_file_M :=
     main.contract_file_M did_manager_string.did_manager_string 15.
 
   Definition contract_file := Eval cbv in (error.extract contract_file_M I).
+
+  (* Definition contract_file_michelson_M := *)
+  (*   main.contract_file_M did_manager_michelson_string.did_manager_michelson_string 30. *)
+
+  (* Definition contract_file_michelson := Eval cbv in (error.extract contract_file_michelson_M I). *)
 End source.
 
 Module annots.
   Import String.
   Definition rotateAuthentication : string := "%rotateAuthentication".
+  Definition rotateOwner : string := "%rotateOwner".
   Definition rotateService : string := "%rotateService".
 End annots.
 
 Definition parameter_ty :=
-  (or (pair
-         (pair address
-               (pair (pair (pair bytes bytes)
-                           (pair bytes key))
-                     nat))
-         signature)
+  (or
+    (or
+      address
       (Some annots.rotateAuthentication)
-      (pair
-         (pair (pair string string)
-               (pair (pair (pair bytes bytes)
-                           (pair bytes key))
-                     nat))
-         signature)
-      (Some annots.rotateService)).
+      address
+      (Some annots.rotateOwner))
+    None
+    (pair string string)
+    (Some annots.rotateService)).
 
 Module did_manager(C:ContractContext).
 
+  (* (pair (pair (big_map %metadata string bytes) (address %owner)) *)
+  (*       (pair (pair %service (string %endpoint) (string %type_)) *)
+  (*             (address %verification_method))). *)
 Definition storage_ty :=
-    pair (pair (pair key (big_map string bytes))
-               (pair nat (pair string string)))
-         address.
+  (pair (pair (big_map string bytes) address)
+        (pair (pair string string) address)).
 
 Definition did_manager : full_contract _ parameter_ty None storage_ty :=
   Eval cbv in contract_file_code source.contract_file.
 
+(* Definition did_manager_michelson : full_contract _ parameter_ty None storage_ty := *)
+(*   Eval cbv in contract_file_code source.contract_file_michelson. *)
+
+
 Module semantics := Semantics C. Import semantics.
 
-Definition did_manager_spec
+Definition did_manager_spec_helper
            (env : @proto_env (Some (parameter_ty, None)))
            (metadata : data (big_map string bytes))
-           (active_key : data key)
-           (rotation_count : data nat)
+           (owner : data address)
            (endpoint : data string)
            (type_ : data string)
            (verification_method : data address)
@@ -85,59 +129,27 @@ Definition did_manager_spec
            (new_storage : data storage_ty)
            (returned_operations : data (list operation)) :=
   let storage : data storage_ty :=
-    ((active_key, metadata),
-     (rotation_count, (endpoint, type_)),
-     verification_method) in
+    ((metadata, owner),
+          ((endpoint, type_), verification_method)) in
 
-  (* %rotateAuthentication: _ *)
+  negb (comparison_to_int (address_compare (sender env) owner) =? 0)%Z = false /\
+  (comparison_to_int (tez.compare (amount env) (0 ~Mutez)) >? 0)%Z = false /\
   match param with
-  | inl ((user, (((chain, digest), (next_digest, user_key)), count)), sig) =>
-    negb
-    (check_signature env active_key sig
-      (pack env
-          (pair
-             (pair (pair (Comparable_type bytes) (Comparable_type bytes))
-                (pair (Comparable_type bytes) key)) 
-             (Comparable_type nat))
-          (chain, digest, (next_digest, user_key), count))) = false /\
-    negb
-      (comparison_to_int
-        (string_compare chain (pack env chain_id (chain_id_ env))) =? 0)%Z = false /\
-    negb (comparison_to_int (count ?= rotation_count + 1)%N =? 0)%Z = false /\
-    (nil, (user_key, metadata, (count, (endpoint, type_)), user), tt) =
+  | inl (inl rotateAuth) =>
+      (nil, (metadata, owner, (endpoint, type_, rotateAuth)), tt) =
       (returned_operations, new_storage, tt)
-
-  (* %rotateService: _ *)
-  | inr (((endpoint_param, type_param),
-        (((current_chain, current_value_digest),
-        (next_value_digest, public_key)), rotation_count_param)), sig) =>
-
-
-    negb
-      (check_signature env active_key sig
-         (pack env
-            (pair
-               (pair (pair (Comparable_type bytes) (Comparable_type bytes))
-                  (pair (Comparable_type bytes) key)) 
-               (Comparable_type nat))
-            (current_chain, current_value_digest,
-            (next_value_digest, public_key), rotation_count_param))) = false /\
-    negb
-      (comparison_to_int
-         (string_compare current_chain (pack env chain_id (chain_id_ env))) =? 0)%Z = false /\
-    negb
-      (comparison_to_int (rotation_count_param ?= rotation_count + 1)%N =? 0)%Z = false /\
-    (nil, (active_key, metadata,
-      (rotation_count_param, (endpoint_param, type_param
-      )), verification_method), tt) =
+  | inl (inr rotateOwner) =>
+      (nil, (metadata, rotateOwner, (endpoint, type_, verification_method)), tt) =
+      (returned_operations, new_storage, tt)
+  | inr rotateService =>
+      (nil, (metadata, owner, (rotateService, verification_method)), tt) =
       (returned_operations, new_storage, tt)
   end.
 
-Lemma did_manager_correct
+Lemma did_manager_spec_helper_correct
       (env : @proto_env (Some (parameter_ty, None)))
       (metadata : data (big_map string bytes))
-      (active_key : data key)
-      (rotation_count : data nat)
+      (owner : data address)
       (endpoint : data string)
       (type_ : data string)
       (verification_method : data address)
@@ -146,13 +158,12 @@ Lemma did_manager_correct
       (returned_operations : data (list operation))
       (fuel : Datatypes.nat) :
   let storage : data storage_ty :=
-    ((active_key, metadata),
-     (rotation_count, (endpoint, type_)),
-     verification_method) in
+    ((metadata, owner),
+          ((endpoint, type_), verification_method)) in
   eval_seq env did_manager (100 + fuel) ((param, storage), tt) =
     Return ((returned_operations, new_storage), tt)
-  <-> did_manager_spec env metadata active_key rotation_count endpoint type_
-        verification_method param new_storage returned_operations.
+  <-> did_manager_spec_helper env metadata owner endpoint type_ verification_method
+    param new_storage returned_operations.
 Proof.
   intro Hfuel.
   remember (100 + fuel) as fuel2.
@@ -160,20 +171,440 @@ Proof.
   rewrite return_precond.
   rewrite eval_seq_precond_correct.
   unfold eval_seq_precond.
-  unfold did_manager_spec.
-  destruct param as [authParams | serviceParams].
-  - simpl.
-    do 4 (more_fuel; simpl).
-    destruct authParams as ((user & (((chain & digest) & (next_digest & user_key)) & count)) & sig).
-    reflexivity.
-  - simpl.
-    do 4 (more_fuel; simpl).
-    destruct serviceParams as (((endpoint_param & type_param) &
-      (((current_chain & current_value_digest) &
-      (next_value_digest & public_key)) & rotation_count_param)) & sig).
-    reflexivity.
+  unfold did_manager_spec_helper.
+  destruct param as [[rotateAuth | rotateOwner] | rotateService];
+  (do 3 (more_fuel; simpl); reflexivity).
 Qed.
+
+(* Lemma did_manager_spec_helper_correct_2 *)
+(*       (env : @proto_env (Some (parameter_ty, None))) *)
+(*       (metadata : data (big_map string bytes)) *)
+(*       (owner : data address) *)
+(*       (endpoint : data string) *)
+(*       (type_ : data string) *)
+(*       (verification_method : data address) *)
+(*       (param : data parameter_ty) *)
+(*       (new_storage : data storage_ty) *)
+(*       (returned_operations : data (list operation)) *)
+(*       (fuel : Datatypes.nat) : *)
+(*   let storage : data storage_ty := *)
+(*     ((metadata, owner), *)
+(*           ((endpoint, type_), verification_method)) in *)
+(*   eval_seq env did_manager_michelson (100 + fuel) ((param, storage), tt) = *)
+(*     Return ((returned_operations, new_storage), tt) *)
+(*   <-> did_manager_spec_helper env metadata owner endpoint type_ verification_method *)
+(*     param new_storage returned_operations. *)
+(* Proof. *)
+(*   intro Hfuel. *)
+(*   remember (100 + fuel) as fuel2. *)
+(*   assert (100 <= fuel2) by lia. *)
+(*   rewrite return_precond. *)
+(*   rewrite eval_seq_precond_correct. *)
+(*   unfold eval_seq_precond. *)
+(*   unfold did_manager_spec_helper. *)
+
+(*   assert (H_negb : forall x, negb x = false <-> x = true). *)
+(*   { *)
+(*     intro x; destruct x; simpl; split; intro H_x; congruence. *)
+(*   } *)
+
+(* (1*   Search (negb _ = _). *1) *)
+(* (1*   Search eq negb. *1) *)
+
+(*   destruct param as [[rotateAuth | rotateOwner] | rotateService]; *)
+(*       idtac. *)
+
+(*     (1* (do 5 (more_fuel; simpl); repeat rewrite H_negb; reflexivity). *1) *)
+
+
+(*   1: { *)
+(*     do 1 (more_fuel; simpl). *)
+(*     do 1 (more_fuel; simpl). *)
+(*     do 1 (more_fuel; simpl). *)
+(*     do 1 (more_fuel; simpl). *)
+(*     do 1 (more_fuel; simpl). *)
+(*     do 1 (more_fuel; simpl). *)
+(*     do 1 (more_fuel; simpl). *)
+(*     do 1 (more_fuel; simpl). *)
+
+(*     repeat rewrite H_negb. *)
+
+
+(*     split; intro H_x. *)
+(*     + clear Heqfuel2; clear H. *)
+(*       repeat match goal with *)
+(*       | H_x : _ /\ _ |- _ => destruct H_x *)
+(*       | H_x : _ = _ |- _ => inversion H_x; destruct H_x *)
+(*       | |- (let (x, y) := ?z in _) => destruct z *)
+(*       end. *)
+(*       congruence. *)
+(*       tauto. *)
+(*     + repeat match goal with *)
+(*       | H_x : (let (x, y) := ?z in _) |- _ => destruct z *)
+(*       | H_x : _ /\ _ |- _ => destruct H_x *)
+(*       end; *)
+(*       repeat split; try congruence; *)
+(*       repeat f_equal; intuition. *)
+
+(*     split; intro H; *) 
+    
+
+(*     (1* rewrite and_iff_compat_l. *1) *)
+
+(*     (1* rewrite <- (and_iff_compat_l (sender env = owner)). *1) *)
+(*     (1* rewrite <- and_iff_compat_l. *1) *)
+(*     (1* Search iff ( _ /\ _). *1) *)
+(*     (1* Check and_pair_eq. *1) *)
+(*     (1* Check and_left. *1) *)
+
+
+(*     reflexivity. *)
+(*     _ *)
+(*     do 1 (more_fuel; simpl). *)
+(*     do 1 (more_fuel; simpl). *)
+(*     do 1 (more_fuel; simpl). *)
+(*     do 1 (more_fuel; simpl). *)
+
+(*     _ *)
+(*   } *)
+
+(*   (do 4 (more_fuel; simpl)). *)
+(*   (do 3 (more_fuel; simpl); intuition). *)
+(* Qed. *)
+
+Definition did_manager_spec
+           (env : @proto_env (Some (parameter_ty, None)))
+           (metadata : data (big_map string bytes))
+           (owner : data address)
+           (endpoint : data string)
+           (type_ : data string)
+           (verification_method : data address)
+           (param : data parameter_ty)
+           (new_storage : data storage_ty)
+           (returned_operations : data (list operation)) :=
+  let storage : data storage_ty :=
+    ((metadata, owner),
+    ((endpoint, type_),
+      verification_method)) in
+
+  match new_storage with
+  | ((new_metadata, new_owner),
+    ((new_endpoint, new_type_),
+      new_verification_method)) =>
+
+    sender env = owner /\
+
+    (* amount env = (0 ~Mutez) /\ *)
+    (int64bv.to_Z (tez.to_int64 (amount env)) <= 0)%Z /\
+
+    returned_operations = nil /\
+    new_metadata = metadata /\
+
+    match param with
+    | inl (inl rotateAuth) =>
+        new_owner = owner /\
+        new_endpoint = endpoint /\
+        new_type_ = type_ /\
+        new_verification_method = rotateAuth
+    | inl (inr rotateOwner) =>
+        new_owner = rotateOwner /\
+        new_endpoint = endpoint /\
+        new_type_ = type_ /\
+        new_verification_method = verification_method
+    | inr (rotateEndpoint, rotateType_) =>
+        new_owner = owner /\
+        new_endpoint = rotateEndpoint /\
+        new_type_ = rotateType_ /\
+        new_verification_method = verification_method
+    end
+  end.
+
+
+Section case_compare_lemmas.
+
+Definition case_compare_Eq ty (s1 s2 : comparable_data ty) :
+  sumbool
+    ( compare ty s1 s2 = Eq /\ s1 = s2 )
+    ( compare ty s1 s2 <> Eq /\ s1 <> s2 ).
+Proof.
+  pose proof (compare_diff ty s1 s2).
+  destruct (compare ty s1 s2) eqn:Hcmp; intuition (try apply compare_eq_iff; congruence).
+Qed.
+
+Definition case_string_compare_Eq (s1 s2 : str) :
+  sumbool
+    ( string_compare s1 s2 = Eq /\ s1 = s2 )
+    ( string_compare s1 s2 <> Eq /\ s1 <> s2 ).
+Proof.
+  replace string_compare with (compare string) by reflexivity.
+  apply case_compare_Eq.
+Qed.
+
+Definition case_tez_compare_Eq (s1 s2 : tez.mutez) :
+  sumbool
+    ( tez.compare s1 s2 = Eq /\ s1 = s2 )
+    ( tez.compare s1 s2 <> Eq /\ s1 <> s2 ).
+Proof.
+  replace tez.compare with (compare mutez) by reflexivity.
+  apply case_compare_Eq.
+Qed.
+
+Definition case_address_compare_Eq (s1 s2 : address_constant) :
+  sumbool
+    ( address_compare s1 s2 = Eq /\ s1 = s2 )
+    ( address_compare s1 s2 <> Eq /\ s1 <> s2 ).
+Proof.
+  replace address_compare with (compare address) by reflexivity.
+  apply case_compare_Eq.
+Qed.
+
+Lemma address_compare_iff (a1 a2 : data address) :
+  negb (comparison_to_int (address_compare a1 a2) =? 0)%Z = false <->
+  a1 = a2.
+Proof.
+  destruct (case_address_compare_Eq a1 a2) as
+    [(str_cmp_eq & str_eq) | (str_cmp_neq & str_neq)].
+  - rewrite str_cmp_eq; tauto.
+  - destruct (address_compare a1 a2); intuition.
+Qed.
+
+End case_compare_lemmas.
+
+
+Lemma tez_not_gt_0 (a1 : tez.mutez) :
+  (comparison_to_int (tez.compare a1 (0 ~Mutez)) >? 0)%Z = false <->
+  (int64bv.to_Z (tez.to_int64 a1) <= 0)%Z.
+Proof.
+  destruct (case_tez_compare_Eq a1 (0 ~Mutez)) as
+    [(str_cmp_eq & str_eq) | (str_cmp_neq & str_neq)].
+  - rewrite str_cmp_eq; simpl.
+    rewrite tez.compare_eq_iff in str_cmp_eq.
+    apply (f_equal (fun x => int64bv.to_Z (tez.to_int64 x))) in str_cmp_eq.
+    replace (int64bv.to_Z (tez.to_int64 (0 ~Mutez)))
+       with (0%Z) in str_cmp_eq.
+    + intuition.
+    + unfold tez.to_int64.
+      match goal with
+      | |- _ = int64bv.to_Z (int64bv.of_Z_safe 0 ?H) =>
+        rewrite (int64bv.of_Z_to_Z_eqv 0 (int64bv.of_Z_safe 0 H));
+        rewrite (int64bv.of_Z_safe_is_of_Z 0 H)
+      end.
+      reflexivity.
+  - pose (cmp := tez.compare a1 (0 ~Mutez)).
+    assert (cmp_eq : tez.compare a1 (0 ~Mutez) = cmp) by reflexivity.
+    rewrite cmp_eq.
+    destruct cmp; try intuition.
+
+    unfold tez.compare in cmp_eq.
+    unfold tez.to_int64 in cmp_eq |- *.
+    unfold int64bv.int64_compare in cmp_eq.
+    unfold int64bv.compare in cmp_eq.
+    rewrite Z.compare_lt_iff in cmp_eq.
+
+    match goal with
+    | cmp_eq : (_ < ?x)%Z |- _ =>
+        assert (x_eq : x = 0%Z)
+    end.
+    + match goal with
+      | |- int64bv.to_Z (int64bv.of_Z_safe 0 ?H) = _ =>
+        rewrite (int64bv.of_Z_to_Z_eqv 0 (int64bv.of_Z_safe 0 H));
+        rewrite (int64bv.of_Z_safe_is_of_Z 0 H)
+      end; reflexivity.
+    + congruence.
+Qed.
+
+
+Lemma did_manager_spec_correct
+      (env : @proto_env (Some (parameter_ty, None)))
+      (metadata : data (big_map string bytes))
+      (owner : data address)
+      (endpoint : data string)
+      (type_ : data string)
+      (verification_method : data address)
+      (param : data parameter_ty)
+      (new_storage : data storage_ty)
+      (returned_operations : data (list operation))
+      (fuel : Datatypes.nat) :
+  let storage : data storage_ty :=
+    ((metadata, owner),
+          ((endpoint, type_), verification_method)) in
+  eval_seq env did_manager (100 + fuel) ((param, storage), tt) =
+    Return ((returned_operations, new_storage), tt)
+  <-> did_manager_spec env metadata owner endpoint type_ verification_method
+    param new_storage returned_operations.
+Proof.
+  Arguments Nat.add : simpl never.
+  simpl.
+  Arguments Nat.add : simpl nomatch.
+
+  rewrite did_manager_spec_helper_correct.
+  unfold did_manager_spec_helper.
+  unfold did_manager_spec.
+
+  rewrite address_compare_iff, tez_not_gt_0.
+
+
+  destruct param as [[rotateAuth | rotateOwner] | rotateService].
+
+  - split; intro H.
+    + repeat match goal with
+      | H : _ /\ _ |- _ => destruct H
+      | H : _ = _ |- _ => inversion H; destruct H
+      | |- (let (x, y) := ?z in _) => destruct z
+      end;
+      tauto.
+    + repeat match goal with
+      | H : (let (x, y) := ?z in _) |- _ => destruct z
+      | H : _ /\ _ |- _ => destruct H
+      end;
+      repeat split; try congruence;
+      repeat f_equal; intuition.
+
+  - split; intro H.
+    + repeat match goal with
+      | H : _ /\ _ |- _ => destruct H
+      | H : _ = _ |- _ => inversion H; destruct H
+      | |- (let (x, y) := ?z in _) => destruct z
+      end;
+      tauto.
+    + repeat match goal with
+      | H : (let (x, y) := ?z in _) |- _ => destruct z
+      | H : _ /\ _ |- _ => destruct H
+      end;
+      repeat split; try congruence;
+      repeat f_equal; intuition.
+
+  - split; intro H.
+    + repeat match goal with
+      | H : _ /\ _ |- _ => destruct H
+      | H : _ = _ |- _ => inversion H; destruct H
+      | |- (let (x, y) := ?z in _) => destruct z
+      end;
+      tauto.
+    + repeat match goal with
+      | H : (let (x, y) := ?z in _) |- _ => destruct z
+      | H : _ /\ _ |- _ => destruct H
+      end;
+      repeat split; try congruence;
+      repeat f_equal; intuition.
+Qed.
+
+      (* ______ *)
+
+  (* _____ *)
+
+  (* - *)
+
+
+      (* f_equal; intuition. *)
+      (* split; try congruence. *)
+      (* intuition tauto. *)
+      (* repeat match goal with *)
+      (* | H : _ = _ |- _ => inversion H; destruct H *)
+      (* end. *)
+      (* tauto. *)
+      (* (1* repeat match goal with *1) *)
+      (* (1* | H : _ /\ _ |- _ => destruct H *1) *)
+      (* (1* end. *1) *)
+      (* (1* destruct H. *1) *)
+    (* rewrite <- (and_iff_compat_l (sender env = owner)). *)
+    (* rewrite <- and_iff_compat_l. *)
+    (* Search iff ( _ /\ _). *)
+    (* Check and_pair_eq. *)
+    (* Check and_left. *)
+    (* Check and_left. *)
+    (* refine (iff_trans (and_left eq_refl (iff_refl _)) _). *)
+    (* refine (iff_trans (and_left eq_refl (iff_refl _)) _). *)
+    (* Search *) 
+    (* Search compare. *)
+    (* _ *)
+
+  (* (1* Search (let (x, y) := _ in _). *1) *)
+  (* _ *)
+
+  (* let (new_metadata_and_owner, new_endpoint_and_verification_method) := new_storage in *)
+  (* let (new_metadata, new_owner) := new_metadata_and_owner in *)
+  (* let (new_endpoint_and_type, new_verification_method) := new_endpoint_and_verification_method in *)
+  (* let (new_endpoint, new_type_) *) 
+
+  (* let ((new_metadata, new_owner), ((new_endpoint, new_type_), new_verification_method)) := new_storage in *)
+  (* let ((new_metadata, new_owner), ((new_endpoint, new_type_), new_verification_method)) := new_storage in *)
+
+
+
+
 
 End did_manager.
 
+(* Check TODO_simplify_raw_spec. *)
+
+
+
+
+
+(*     Arguments compare : simpl never.    (1* do not unfold compare *1) *)
+(*     Arguments tez.mutez : simpl never. *)
+(*     Arguments comparable_data : simpl never. *)
+(*     Arguments simple_comparable_data : simpl never. *)
+(*     Arguments data_to_comparable_data : simpl never. *)
+(*     Arguments concrete_data_to_data : simpl never. *)
+
+(*     Arguments int64bv.of_Z_safe : simpl never. *)
+(*     (1* Arguments Comparable_constant : simpl never. *1) *)
+
+(*     (1* Locate "~". *1) *)
+(*     (1* Search Mutez. *1) *)
+(*     (1* :Notation "n ~mutez" := (Comparable_constant mutez (n ~Mutez)) (at level 100). *1) *)
+
+
+(*     Opaque int64bv.int64. *)
+(*     Opaque tez.mutez. *)
+
+(*     (1* Print data_to_comparable_data. *1) *)
+(*     (1* Print simple_comparable_data. *1) *)
+(*     (1* Search simple_comparable_type. *1) *)
+(*     (1* Print Comparable_type_simple. *1) *)
+(*     (1* Print Comparable_type_simpl. *1) *)
+
+
+(*     (1* Print tez.mutez. *1) *)
+(*     (1* Print simple_comparable_data. *1) *)
+(*     (1* Search mutez. *1) *)
+(*     (1* simpl. *1) *)
+
+(*     destruct env. *)
+(*     simpl. *)
+
+(*     (1* do 1 (more_fuel; simpl). *1) *)
+(*     do 3 (more_fuel; simpl). *)
+
+(*     _ *)
+
+(*     fold (int64bv.of_Z_safe 0 eq_refl). *)
+(*     fold (0 ~Mutez). *)
+
+(*     Transparent tez.mutez. *)
+(*     fold tez.mutez. *)
+(*     fold tez.mutez. *)
+
+(*     _ *)
+(*     fold tez.mutez. *)
+
+(*     _ *)
+(*     simpl. *)
+(*     Arguments compare : simpl nomatch.  (1* unfold if extra simplification is possible *1) *)
+
+
+(*     Check compare. *)
+(*     Locate eval_seq_precond. *)
+(*     Locate compare. *)
+(*     Search mutez. *)
+(*     Search COMPARE. *)
+(*     Print eval_seq_precond_body_aux. *)
+(*     Print eval_seq_precond_body. *)
+(*     Print eval_precond. *)
+(*     Print eval_seq_precond. *)
+(*     simpl. *)
+(*     _ *)
+(*   } *)
 
